Also expose bind and return but still no dice

rupicola/io/RunningExample.fst
@@ -49,14 +49,33 @@ unfold
 let hist_prepost #a (pre : hist_pre) (post : (h:_ -> hist_post h a)) : hist a =
   fun h p -> pre h /\ (forall r lt. post h lt r ==> p lt r)
 
+unfold
 let wrapper_spec (f task : string) =
-  hist_prepost (* Should I use to_hist? *)
-    (fun h -> False)
+  hist_prepost
+    (fun h -> True)
     (fun h lt r -> True)
 
 let wrapper_sat_spec f task agent :
-  Lemma (theta (wrapper f task agent) ⊑ wrapper_spec f task)
-= ()
+  Lemma (theta_unf (wrapper f task agent) ⊑ wrapper_spec f task)
+  // by (norm [delta_only [`%theta_unf;`%wrapper;`%(let!@!);`%(let!@);`%io_bind]] ; (* compute () ; *) explode () ; dump "oh")
+= // unfold_theta #(resexn unit)
+  introduce
+    forall (h: Trace.history) (p: hist_post h (resexn unit)).
+      (forall (r: resexn unit) (lt: Trace.local_trace h). p lt r) ==>
+      theta_unf (wrapper f task agent) h p
+  with begin
+    introduce
+      (forall (r: resexn unit) (lt: Trace.local_trace h). p lt r) ==>
+      theta_unf (wrapper f task agent) h p
+    with _. begin
+      admit ()
+    end
+  end
+  // ()
+
+// assume (forall (h: Trace.history) (p: hist_post h (resexn unit)).
+//       (forall (r: resexn unit) (lt: Trace.local_trace h). auto_squash (p lt r)) ==>
+//       theta (wrapper f task agent) h p)
 
 // val wrapped_wrapper : progS wrapper_intS
 // let wrapped_wrapper =
